

Consider systems of the form
%\newcommand{\xpt}[1]{\mathcal{E}_t \left ( #1 \right ) }
\newcommand{\xpt}[1]{#1}
\begin{gather}
\sum_{i=-\tau}^\theta H_i x_{t+i} =
\begin{bmatrix}
\psi_\epsilon & \psi_z  
\end{bmatrix}
  \begin{bmatrix}
\epsilon_t \\\xpt{z_{t}(x_{t-1},\epsilon_t) }   
  \end{bmatrix}
  \,\,\forall t. \intertext{Solutions will take the form\citep{anderson10}}
  x_t=B x_{t-1}+ \phi \psi_\epsilon\epsilon_t + \sum_{s=0}^\infty F^s \phi \psi_z 
\xpt{z_{t+s}(x_{t+s-1},\epsilon_t)    } \label{myEqn}
% \intertext{ if $z_{t+s}=z^\ast, \forall s$}
%   x_t=B x_{t-1}+(z_t(x_{t-1},\epsilon_t) - \xpt{z^\ast(x_{t-1},\epsilon_{t+s})}(I-F)^{-1} \phi \psi
%   \begin{bmatrix}
% \epsilon_t \\z^\ast(x_{t-1},\epsilon_t)    
%   \end{bmatrix}\intertext{ if $z_{t+s}=z^\ast, \forall s$}
\end{gather}
To accommodate inequality constraints of the form
\begin{gather*}
  x_t \ge \bar{x}
\end{gather*}

\noindent
we will determine a sequence of $z_t$ that 
will allow us to  impose the constraints over successively longer time periods.
